Work towards simpler initialization code
The goal is for the missing partition lemmas to have easier proofs that
do not involve painstaking analysis of relatively involved, "stateful"
(in the sense of cumulative effects) when a simpler scheme will suffice.
This seems fairly easy up to reserve_component_blocks at least. The
obvious small inefficiency being introduced by the reuse of existing
code is the need to unzip the final result.

Intermediate/Machine.v
@@ -491,6 +491,29 @@ Definition prepare_procedures (p: program) (mem: Memory.t)
   : Memory.t * NMap (NMap code) * EntryPoint.t :=
   reserve_procedure_blocks p (mem, emptym, emptym) (elementsm (prog_procedures p)).
 
+(* For each component, integrate the (now separate) fetching of its procedures,
+   obtention of its initial component memory and then reserve_component_blocks.
+   The logic of reserve_procedure_blocks is implicit in the map-like nature of
+   its results. Then, decompose the results, composed as a whole in the result
+   of reserving component blocks, turning a map of triples into a triple of
+   identically indexed maps. *)
+Definition prepare_procedures_initial_memory (p: program)
+  : Memory.t * NMap (NMap code) * EntryPoint.t :=
+  let m :=
+      mkfmapf
+        (fun C =>
+           let Cprocs := odflt emptym ((prog_procedures p) C) in
+           let Cmem := ComponentMemory.prealloc (odflt emptym ((prog_buffers p) C)) in
+           reserve_component_blocks p C (Cmem, emptym, emptym) (elementsm Cprocs))
+        (domm (prog_interface p)) in
+  (mapm (fun x => fst (fst x)) m, mapm (fun x => snd (fst x)) m, mapm snd m).
+
+(* We want to ensure something like this:
+     Goal
+       forall p, prepare_procedures_initial_memory p =
+                 prepare_procedures p (prepare_initial_memory p).
+  Possibly assuming the well-formedness of the program. *)
+
 (* initialization of the empty program *)
 
 Theorem prepare_initial_memory_empty_program:
